code/ecdsap256/Hacl.P256.fst
@@ -83,11 +83,3 @@ let ecp256dh_r result pubKey scalar = Hacl.Impl.P256.DH.ecp256dh_r result pubKey
 let is_more_than_zero_less_than_order x =
   Hacl.Impl.P256.Signature.Common.isMoreThanZeroLessThanOrder x
  *) 
-
-
-
-
-
-let pointAddMixed result p q =  Hacl.Impl.P256.MixedPointAdd.pointAddMixed result p q
-
-let do_lookup a scalar = Hacl.Impl.P256.Q.CR.do_lookup a scalar
